bq proof

compcertox/BQspec.v
@@ -8,479 +8,358 @@ From compcert Require Import
      Smallstep SimplLocalsproof.
 (* From cal.example Require Import BQ. *)
 Import ListNotations.
-From compcertox Require Import Lifting BQcode.
+From compcertox Require Import Lifting BQcode RBspec.
 
-Definition rb_state : Type := (nat -> val) * nat * nat.
+Inductive sig := enq | deq.
 
-Inductive sig := inc1 | inc2 | geti | seti.
-
-Inductive rb_internal_state: Type :=
-| rb_init: forall (sig: sig) (s: rb_state) (vs: list val) (m: mem), rb_internal_state
-| rb_final: forall (s: rb_state) (v: val) (m: mem), rb_internal_state.
+Inductive bq_internal_state: Type :=
+| bq_init: forall (sig: sig) (vs: list val) (m: mem), bq_internal_state
+| bq_call: forall (sig: RBspec.sig) (vs: list val) (m: mem), bq_internal_state
+| bq_middle: forall (sig: sig) (vs: list val) (m: mem), bq_internal_state
+| bq_middle': forall (sig: sig) (vs: val) (m: mem), bq_internal_state
+| bq_final: forall (v: val) (m: mem), bq_internal_state.
 
 Section RB_LTS.
 
   Variable ge:  genv.
 
-  Inductive rb_initial_state: c_query * rb_state -> rb_internal_state -> Prop :=
-  | initial_state_inc1: forall vf b m rbst sig,
+  Inductive bq_initial_state: c_query -> bq_internal_state -> Prop :=
+  | initial_state_geti: forall vf b v m  sig,
       vf = Vptr b Integers.Ptrofs.zero ->
-      Genv.find_symbol ge inc1_id = Some b ->
-      Ple (Genv.genv_next ge) (Mem.nextblock m) ->
-      sig = inc1_sg ->
-      rb_initial_state (cq vf sig nil m, rbst) (rb_init inc1 rbst nil m)
-  | initial_state_inc2: forall vf b m rbst sig,
-      vf = Vptr b Integers.Ptrofs.zero ->
-      Genv.find_symbol ge inc2_id = Some b ->
-      Ple (Genv.genv_next ge) (Mem.nextblock m) ->
-      sig = inc2_sg ->
-      rb_initial_state (cq vf sig nil m, rbst) (rb_init inc2 rbst nil m)
-  | initial_state_geti: forall vf b v m rbst sig,
-      vf = Vptr b Integers.Ptrofs.zero ->
-      Genv.find_symbol ge get_id = Some b ->
+      Genv.find_symbol ge enq_id = Some b ->
       Ple (Genv.genv_next ge) (Mem.nextblock m) ->
       Cop.val_casted v tint ->
-      sig = get_sg ->
-      rb_initial_state (cq vf sig [v] m, rbst) (rb_init geti rbst [v] m)
-  | initial_state_seti: forall vf b m rbst sig vargs v1 v2,
+      sig = enq_sg ->
+      bq_initial_state (cq vf sig [v] m) (bq_init enq [v] m)
+  | initial_state_seti: forall vf b m  sig,
       vf = Vptr b Integers.Ptrofs.zero ->
-      Genv.find_symbol ge set_id = Some b ->
+      Genv.find_symbol ge deq_id = Some b ->
       Ple (Genv.genv_next ge) (Mem.nextblock m) ->
-      sig = set_sg ->
-      vargs = [ v1; v2 ] ->
-      Cop.val_casted v1 tint ->
-      Cop.val_casted v2 tint ->
-      rb_initial_state (cq vf sig vargs m, rbst) (rb_init seti rbst vargs m).
+      sig = deq_sg ->
+      bq_initial_state (cq vf sig nil m) (bq_init deq  nil m).
 
-  Inductive rb_final_state: rb_internal_state -> c_reply * rb_state -> Prop :=
-  | final_state: forall rv m rbst,
-      rb_final_state (rb_final rbst rv m) (cr rv m, rbst).
+  Inductive bq_final_state: bq_internal_state -> c_reply -> Prop :=
+  | final_state: forall rv m,
+      bq_final_state (bq_final rv m) (cr rv m).
 
-  Inductive rb_step: rb_internal_state -> trace -> rb_internal_state -> Prop :=
-  | inc1_step:
-    forall f c1 c2 m v,
-      v = Vint (Integers.Int.repr (Z.of_nat c1)) ->
-      rb_step (rb_init inc1 (f, c1, c2) nil m) E0 (rb_final (f, (S c1 mod N)%nat, c2) v m)
-  | inc2_step:
-    forall f c1 c2 m v,
-      v = Vint (Integers.Int.repr (Z.of_nat c2)) ->
-      rb_step (rb_init inc2 (f, c1, c2) nil m) E0 (rb_final (f, c1, (S c2 mod N)%nat) v m)
-  | get_step:
-    forall f c1 c2 m v i,
-      v = Vint (Integers.Int.repr (Z.of_nat i)) ->
-      (i < N)%nat ->
-      rb_step (rb_init geti (f, c1, c2) [v] m) E0 (rb_final (f, c1, c2) (f i) m)
-  | set_step:
-    forall f c1 c2 m v1 v2 i,
-      v1 = Vint (Integers.Int.repr (Z.of_nat i)) ->
-      (i < N)%nat ->
-      Cop.val_casted v2 tint ->
-      rb_step (rb_init seti (f, c1, c2) [v1; v2] m) E0
-        (rb_final ((fun j => if Nat.eq_dec i j then v2 else f j), c1, c2)
-                  Vundef m).
+  Inductive bq_step: bq_internal_state -> trace -> bq_internal_state -> Prop :=
+  | enq_step1 v m:
+      bq_step (bq_init enq [v] m) E0 (bq_call RBspec.inc2 [v] m)
+  | enq_step2 v1 v2 m:
+      bq_step (bq_middle enq [v1; v2] m) E0 (bq_call RBspec.seti [v1; v2] m)
+  | enq_step3 vs m:
+      bq_step (bq_middle' enq vs m) E0 (bq_final Vundef m)
+  | deq_step1 m:
+      bq_step (bq_init deq [] m) E0 (bq_call RBspec.inc1 [] m)
+  | deq_step2 v m:
+      bq_step (bq_middle deq [v] m) E0 (bq_call RBspec.geti [v] m)
+  | deq_step3 v m:
+      bq_step (bq_middle' deq v m) E0 (bq_final v m).
 
-  Program Definition rb_lts: lts li_c (li_c@rb_state) rb_internal_state :=
+  Inductive bq_at_external: bq_internal_state -> c_query -> Prop :=
+  | bq_ext_inc1 vf sig vs m b:
+    vf = Vptr b Integers.Ptrofs.zero ->
+    Genv.find_symbol ge inc1_id = Some b ->
+    sig = inc1_sg ->
+    bq_at_external (bq_call RBspec.inc1 vs m) (cq vf sig nil m)
+  | bq_ext_inc2 vf sig vs m b:
+    vf = Vptr b Integers.Ptrofs.zero ->
+    Genv.find_symbol ge inc2_id = Some b ->
+    sig = inc2_sg ->
+    bq_at_external (bq_call RBspec.inc2 vs m) (cq vf sig nil m)
+  | bq_ext_get vf sig v m b:
+    vf = Vptr b Integers.Ptrofs.zero ->
+    Genv.find_symbol ge get_id = Some b ->
+    sig = get_sg ->
+    bq_at_external (bq_call RBspec.geti [v] m) (cq vf sig [v] m)
+  | bq_ext_set vf sig vs m b:
+    vf = Vptr b Integers.Ptrofs.zero ->
+    Genv.find_symbol ge set_id = Some b ->
+    sig = set_sg ->
+    bq_at_external (bq_call RBspec.seti vs m) (cq vf sig vs m).
+
+  Inductive bq_after_external: bq_internal_state -> c_reply -> bq_internal_state -> Prop :=
+  | bq_aft_inc1 rv m :
+    Cop.val_casted rv tint ->
+    bq_after_external (bq_call RBspec.inc1 nil m) (cr rv m) (bq_middle deq [rv] m)
+  | bq_aft_inc2 rv v m :
+    Cop.val_casted rv tint ->
+    bq_after_external (bq_call RBspec.inc2 [v] m) (cr rv m) (bq_middle enq [rv; v] m)
+  | bq_aft_get rv vs m :
+    Cop.val_casted rv tint ->
+    bq_after_external (bq_call RBspec.geti vs m) (cr rv m) (bq_middle' deq rv m)
+  | bq_aft_set vs m :
+    bq_after_external (bq_call RBspec.seti vs m) (cr Vundef m) (bq_middle' enq Vundef m).
+
+  Program Definition bq_lts: lts li_c li_c bq_internal_state :=
     {|
       Smallstep.genvtype := genv;
-      Smallstep.step ge := rb_step;
-      Smallstep.initial_state := rb_initial_state;
-      Smallstep.at_external _ _ := False;
-      Smallstep.after_external _ _ _ := False;
-      Smallstep.final_state := rb_final_state;
+      Smallstep.step ge := bq_step;
+      Smallstep.initial_state := bq_initial_state;
+      Smallstep.at_external := bq_at_external;
+      Smallstep.after_external := bq_after_external;
+      Smallstep.final_state := bq_final_state;
       Smallstep.globalenv := ge;
     |}.
 
 End RB_LTS.
 
-Definition rb_spec: semantics li_c (li_c@rb_state) :=
+Definition bq_spec: semantics li_c li_c :=
   {|
-    skel := AST.erase_program rb_program;
-    activate se := rb_lts (Clight.globalenv se rb_program);
-    footprint := AST.footprint_of_program rb_program;
+    skel := AST.erase_program bq_program;
+    activate se := bq_lts (Clight.globalenv se bq_program);
+    footprint := AST.footprint_of_program bq_program;
   |}.
 
-Inductive nat_rel: nat -> val -> Prop :=
-| nat_rel_intro n i:
-  Z.of_nat n = Integers.Int.intval i ->
-  nat_rel n (Vint i).
+Inductive bq_ms se: bq_internal_state -> Clight.state -> Prop :=
+| bq_ms_enq:
+  forall vf m v,
+    Cop.val_casted v tint ->
+    Genv.find_funct (Genv.globalenv se bq_program) vf = Some (Internal bq_enq) ->
+    bq_ms se (bq_init enq [v] m) (Callstate vf [v] Kstop m)
+| bq_ms_deq:
+  forall vf m,
+    Genv.find_funct (Genv.globalenv se bq_program) vf = Some (Internal bq_deq) ->
+    bq_ms se (bq_init deq [] m) (Callstate vf [] Kstop m)
 
-Inductive rel_cnt se (id: positive): nat -> mem -> Prop :=
-| rel_cnt_intro b v n m:
-  Genv.find_symbol se id = Some b ->
-  Mem.load Mint32 m b 0 = Some v ->
-  nat_rel n v -> (n < N)%nat ->
-  Mem.range_perm m b 0 4 Cur Writable ->
-  rel_cnt se id n m.
+| bq_ms_call_inc1:
+  forall vf k m b,
+    vf = Vptr b Integers.Ptrofs.zero ->
+    Genv.find_symbol se inc1_id = Some b ->
+    k = (Kcall (Some bq_deq_tmp1) bq_deq empty_env
+          (PTree.Node (PTree.Node PTree.Leaf (Some Vundef) PTree.Leaf) (Some Vundef) PTree.Leaf)
+          (Kseq
+             (Ssequence
+                (Scall (Some bq_deq_tmp2) (Evar get_id (Tfunction (Tcons tint Tnil) tint cc_default))
+                   [Etempvar bq_deq_tmp1 tint]) (Sreturn (Some (Etempvar bq_deq_tmp2 tint)))) Kstop)) ->
+    bq_ms se (bq_call RBspec.inc1 [] m) (Callstate vf [] k m)
+| bq_ms_call_inc2:
+  forall vf k m v b,
+    Cop.val_casted v tint ->
+    vf = Vptr b Integers.Ptrofs.zero ->
+    Genv.find_symbol se inc2_id = Some b ->
+    k = (Kcall (Some bq_enq_tmp) bq_enq empty_env
+          (PTree.Node (PTree.Node PTree.Leaf (Some Vundef) PTree.Leaf) (Some v) PTree.Leaf)
+          (Kseq
+             (Ssequence
+                (Scall None (Evar set_id (Tfunction (Tcons tint (Tcons tint Tnil)) tvoid cc_default))
+                   [Etempvar bq_enq_tmp tint; Etempvar enq_arg_id tint]) (Sreturn None)) Kstop)) ->
+    bq_ms se (bq_call RBspec.inc2 [v] m) (Callstate vf [] k m)
 
-Inductive rel_arr se : (nat -> val) -> mem -> Prop :=
-| rel_arr_intro f b m:
-  Genv.find_symbol se arr_id = Some b ->
-  (forall i, (i < N)%nat ->
-        exists v, Mem.load Mint32 m b (4 * Z.of_nat i) = Some v /\ (f i) = v /\ Cop.val_casted v tint) ->
-  (forall ofs, 0 <= ofs < 4 * Nz -> Mem.perm m b ofs Cur Writable) ->
-  rel_arr se f m.
+| bq_ms_mid_enq:
+  forall m v1 v2 k,
+    Cop.val_casted v1 tint ->
+    Cop.val_casted v2 tint ->
+    k = (Kcall (Some bq_enq_tmp) bq_enq empty_env
+          (PTree.Node (PTree.Node PTree.Leaf (Some Vundef) PTree.Leaf) (Some v2) PTree.Leaf)
+          (Kseq
+             (Ssequence
+                (Scall None (Evar set_id (Tfunction (Tcons tint (Tcons tint Tnil)) tvoid cc_default))
+                   [Etempvar bq_enq_tmp tint; Etempvar enq_arg_id tint]) (Sreturn None)) Kstop)) ->
+    bq_ms se (bq_middle enq [v1; v2] m) (Returnstate v1 k m)
+| bq_ms_mid_deq:
+  forall m v k,
+    Cop.val_casted v tint ->
+    k = (Kcall (Some bq_deq_tmp1) bq_deq empty_env
+          (PTree.Node (PTree.Node PTree.Leaf (Some Vundef) PTree.Leaf) (Some Vundef) PTree.Leaf)
+          (Kseq
+             (Ssequence
+                (Scall (Some bq_deq_tmp2) (Evar get_id (Tfunction (Tcons tint Tnil) tint cc_default))
+                   [Etempvar bq_deq_tmp1 tint]) (Sreturn (Some (Etempvar bq_deq_tmp2 tint)))) Kstop)) ->
+    bq_ms se (bq_middle deq [v] m) (Returnstate v k m)
 
-Inductive rb_match_mem: Genv.symtbl -> rb_state -> mem -> Prop :=
-| rb_match_mem_intro:
-  forall se f c1 c2 m,
-    rel_cnt se cnt1_id c1 m ->
-    rel_cnt se cnt2_id c2 m ->
-    rel_arr se f m ->
-    rb_match_mem se (f, c1, c2) m.
+| bq_ms_call_get:
+  forall vf k m v b,
+    vf = Vptr b Integers.Ptrofs.zero ->
+    Genv.find_symbol se get_id = Some b ->
+    Cop.val_casted v tint ->
+    k = (Kcall (Some bq_deq_tmp2) bq_deq empty_env
+          (PTree.Node (PTree.Node PTree.Leaf (Some Vundef) PTree.Leaf) (Some v) PTree.Leaf)
+          (Kseq (Sreturn (Some (Etempvar bq_deq_tmp2 tint))) Kstop)) ->
+    bq_ms se (bq_call RBspec.geti [v] m) (Callstate vf [v] k m)
+| bq_ms_call_set:
+  forall vf k m v1 v2 b,
+    vf = Vptr b Integers.Ptrofs.zero ->
+    Genv.find_symbol se set_id = Some b ->
+    Cop.val_casted v1 tint ->
+    Cop.val_casted v2 tint ->
+    k = (Kcall None bq_enq empty_env (PTree.Node (PTree.Node PTree.Leaf (Some v1) PTree.Leaf) (Some v2) PTree.Leaf) (Kseq (Sreturn None) Kstop)) ->
+    bq_ms se (bq_call RBspec.seti [v1; v2] m) (Callstate vf [v1; v2] k m)
 
-Inductive rb_match_query: Genv.symtbl -> c_query * rb_state -> c_query -> Prop :=
-| rb_query_intro:
-  forall se m vf sig vargs rbst,
-    rb_match_mem se rbst m ->
-    rb_match_query se (cq vf sig vargs m, rbst) (cq vf sig vargs m).
+| bq_ms_mid'_enq:
+  forall m v k le,
+    k = (Kcall None bq_enq empty_env le (Kseq (Sreturn None) Kstop)) ->
+    bq_ms se (bq_middle' enq v m) (Returnstate v k m)
+| bq_ms_mid'_deq:
+  forall m v rv k,
+    Cop.val_casted rv tint ->
+    Cop.val_casted v tint ->
+    k = (Kcall (Some bq_deq_tmp2) bq_deq empty_env
+          (PTree.Node (PTree.Node PTree.Leaf (Some Vundef) PTree.Leaf) (Some v) PTree.Leaf)
+          (Kseq (Sreturn (Some (Etempvar bq_deq_tmp2 tint))) Kstop)) ->
+    bq_ms se (bq_middle' deq rv m) (Returnstate rv k m)
 
-Inductive rb_match_reply: Genv.symtbl -> c_reply * rb_state -> c_reply -> Prop :=
-| rb_reply_intro:
-  forall se rbst m m' rv,
-    rb_match_mem se rbst m' ->
-    rb_match_reply se (cr rv m, rbst) (cr rv m').
+| bq_ms_final:
+  forall rv m,
+    bq_ms se (bq_final rv m) (Returnstate rv Kstop m).
 
-Program Definition rb_cc: callconv (li_c@rb_state) li_c :=
-  {|
-    ccworld := Genv.symtbl;
-    match_senv se se1 se2 := se = se1 /\ se = se2;
-    match_query := rb_match_query;
-    match_reply := rb_match_reply;
-  |}.
-Next Obligation. reflexivity. Qed.
-Next Obligation. inv H0. reflexivity. Qed.
-Next Obligation. inv H. reflexivity. Qed.
+Import Ptrofs.
 
-Inductive rb_ms se: rb_internal_state -> Clight.state -> Prop :=
-| rb_ms_inc1:
-  forall vf  m rbst vs,
-    rb_match_mem se rbst m ->
-    Genv.find_funct (Genv.globalenv se rb_program) vf = Some (Internal rb_inc1) ->
-    rb_ms se  (rb_init inc1 rbst vs m) (Callstate vf vs Kstop m)
-| rb_ms_inc2:
-  forall vf  m rbst vs,
-    rb_match_mem se rbst m ->
-    Genv.find_funct (Genv.globalenv se rb_program) vf = Some (Internal rb_inc2) ->
-    rb_ms se  (rb_init inc2 rbst vs m) (Callstate vf vs Kstop m)
-| rb_ms_set:
-  forall vf  m rbst vs,
-    rb_match_mem se rbst m ->
-    Genv.find_funct (Genv.globalenv se rb_program) vf = Some (Internal rb_set) ->
-    rb_ms se  (rb_init seti rbst vs m) (Callstate vf vs Kstop m)
-| rb_ms_get:
-  forall vf  m rbst vs,
-    rb_match_mem se rbst m ->
-    Genv.find_funct (Genv.globalenv se rb_program) vf = Some (Internal rb_get) ->
-    rb_ms se  (rb_init geti rbst vs m) (Callstate vf vs Kstop m)
-| rb_ms_final:
-  forall rv m m' rbst,
-    rb_match_mem se rbst m' ->
-    rb_ms se (rb_final rbst rv m) (Returnstate rv Kstop m').
+Lemma inc2_block se:
+  Genv.valid_for (erase_program bq_program) se ->
+  exists b, Genv.find_symbol (globalenv ((semantics2 bq_program) se)) inc2_id = Some b /\
+         Genv.find_funct (globalenv ((semantics2 bq_program) se)) (Vptr b zero) = Some inc2_ext.
+Proof.
+  intros Hse. eapply Genv.find_def_symbol with (id := inc2_id) in Hse .
+  edestruct (proj1 Hse) as (b & Hb1 & Hb2). reflexivity.
+  exists b. split; eauto. eapply genv_funct_symbol; eauto.
+Qed.
+
+Lemma set_block se:
+  Genv.valid_for (erase_program bq_program) se ->
+  exists b, Genv.find_symbol (globalenv ((semantics2 bq_program) se)) set_id = Some b /\
+         Genv.find_funct (globalenv ((semantics2 bq_program) se)) (Vptr b zero) = Some set_ext.
+Proof.
+  intros Hse. eapply Genv.find_def_symbol with (id := set_id) in Hse .
+  edestruct (proj1 Hse) as (b & Hb1 & Hb2). reflexivity.
+  exists b. split; eauto. eapply genv_funct_symbol; eauto.
+Qed.
+
+Lemma inc1_block se:
+  Genv.valid_for (erase_program bq_program) se ->
+  exists b, Genv.find_symbol (globalenv ((semantics2 bq_program) se)) inc1_id = Some b /\
+         Genv.find_funct (globalenv ((semantics2 bq_program) se)) (Vptr b zero) = Some inc1_ext.
+Proof.
+  intros Hse. eapply Genv.find_def_symbol with (id := inc1_id) in Hse .
+  edestruct (proj1 Hse) as (b & Hb1 & Hb2). reflexivity.
+  exists b. split; eauto. eapply genv_funct_symbol; eauto.
+Qed.
+
+Lemma get_block se:
+  Genv.valid_for (erase_program bq_program) se ->
+  exists b, Genv.find_symbol (globalenv ((semantics2 bq_program) se)) get_id = Some b /\
+         Genv.find_funct (globalenv ((semantics2 bq_program) se)) (Vptr b zero) = Some get_ext.
+Proof.
+  intros Hse. eapply Genv.find_def_symbol with (id := get_id) in Hse .
+  edestruct (proj1 Hse) as (b & Hb1 & Hb2). reflexivity.
+  exists b. split; eauto. eapply genv_funct_symbol; eauto.
+Qed.
+Opaque Genv.find_funct semantics2.
 
 Opaque semantics2.
 Opaque Nat.modulo.
 Require Import Lia.
 
-Lemma rel_cnt_store_other:
-  forall se i j c m b m' v ofs,
-  i <> j ->
-  rel_cnt se i c m ->
-  Genv.find_symbol se j = Some b ->
-  Mem.store Mint32 m b ofs v = Some m' ->
-  rel_cnt se i c m'.
-Proof.
-  intros. inv H0.
-  assert (b <> b0).
-  { intros <-. exploit Genv.find_symbol_injective.
-    apply H1. apply H3. intros <-. apply H. easy. }
-  econstructor; eauto.
-  erewrite Mem.load_store_other; eauto.
-  intros ofs' Hofs. eapply Mem.perm_store_1; eauto.
-Qed.
-
-Lemma rel_arr_store_other:
-  forall se j f m b m' v ofs',
-  j <> arr_id ->
-  rel_arr se f m ->
-  Genv.find_symbol se j = Some b ->
-  Mem.store Mint32 m b ofs' v = Some m' ->
-  rel_arr se f m'.
-Proof.
-  intros. inv H0.
-  assert (b <> b0).
-  { intros <-. exploit Genv.find_symbol_injective.
-    apply H1. apply H3. intros ->. apply H. easy. }
-  econstructor; eauto.
-  intros. specialize (H4 _ H6). destruct H4 as (? & ? & ? & ?). subst.
-  eexists; repeat split; eauto.
-  erewrite Mem.load_store_other; eauto.
-  intros ofs Hofs. eapply Mem.perm_store_1; eauto.
-Qed.
-
-Lemma cnt_inc_simp c i:
-  Z.of_nat c = Int.intval i -> (c < N)%nat ->
-  Z.of_nat (S c mod N) = Int.intval (Int.modu (Int.add i (Int.repr 1)) (Int.repr Nz)).
-Proof.
-  intros H1 H2. unfold Int.add, Int.modu.
-  apply inj_le in H2. rewrite Nat2Z.inj_succ in H2.
-  rewrite H1 in H2.
-  repeat rewrite Int.unsigned_repr.
-  all: unfold Nz in *; cbn -[Z.mul] in *; unfold Int.unsigned; try lia.
-  - unfold Int.unsigned. rewrite <- H1.
-    rewrite mod_Zmod.
-    + f_equal. rewrite Nat2Z.inj_succ. reflexivity.
-    + unfold N. lia.
-  - unfold Int.unsigned. rewrite <- H1.
-    exploit (Z.mod_pos_bound (Z.of_nat c + 1) (Z.of_nat N)); unfold N; lia.
-Qed.
-
-Lemma cop_sem_mod m i j:
-  j <> Int.zero -> Cop.sem_mod (Vint i) tint (Vint j) tint m = Some (Vint (Int.modu i j)).
-Proof.
-  intros Hj. unfold Cop.sem_mod.
-  unfold Cop.sem_binarith. cbn.
-  unfold Cop.sem_cast. cbn.
-  destruct Archi.ptr64. cbn.
-  rewrite Int.eq_false; eauto.
-  rewrite Int.eq_false; eauto.
-Qed.
-
-Lemma Nbound : 4 * Nz <= Ptrofs.max_unsigned. Admitted.
-Lemma Nbound' : 4 * Nz <= Int.max_unsigned. Admitted.
-
-Lemma rb_correct: forward_simulation cc_id rb_cc rb_spec (Clight.semantics2 rb_program).
+Lemma bq_correct: forward_simulation cc_id cc_id bq_spec (Clight.semantics2 bq_program).
 Proof.
   constructor. econstructor. reflexivity. firstorder.
   intros. instantiate (1 := fun _ _ _ => _). cbn beta.
   destruct H. subst.
-  set (ms := fun (s1: state rb_spec) s2 => rb_ms se2 s1 s2).
+  set (ms := fun (s1: state bq_spec) s2 => bq_ms se1 s1 s2).
   eapply forward_simulation_plus with (match_states := ms).
   - intros. destruct q1. inv H. inv H1.
     + eexists. split.
       * econstructor; eauto.
         eapply genv_funct_symbol; eauto. reflexivity.
         unfold type_of_function. f_equal; cbn.
-        constructor.
-      * apply rb_ms_inc1; eauto.
-        eapply genv_funct_symbol; eauto.
-    + eexists. split.
-      * econstructor; eauto.
-        eapply genv_funct_symbol; eauto. reflexivity.
-        unfold type_of_function. f_equal; cbn.
-        constructor.
-      * apply rb_ms_inc2; eauto.
-        eapply genv_funct_symbol; eauto.
-    + eexists. split.
-      * econstructor; eauto.
-        eapply genv_funct_symbol; eauto. reflexivity.
-        unfold type_of_function. f_equal; cbn.
         constructor; eauto. constructor.
-      * apply rb_ms_get; eauto.
-        eapply genv_funct_symbol; eauto.
+      * constructor; eauto. eapply genv_funct_symbol; eauto.
     + eexists. split.
       * econstructor; eauto.
         eapply genv_funct_symbol; eauto. reflexivity.
         unfold type_of_function. f_equal; cbn.
-        constructor; eauto. constructor; eauto. constructor.
-      * apply rb_ms_set; eauto.
-        eapply genv_funct_symbol; eauto.
+        constructor; eauto.
+      * constructor. eapply genv_funct_symbol; eauto.
   - intros. destruct r1. inv H1. inv H.
-    eexists. split. constructor. constructor. eauto.
-  - intros. inv H1.
+    eexists. split. constructor. constructor.
   - intros. inv H1; inv H.
     (* inc1 *)
-    + inv H2. inv H6. inv H2.
-      edestruct (Mem.valid_access_store m Mint32 b 0) as (m' & Hm').
-      {
-        constructor.
-        - intros ofs Hofs. apply H5. cbn [size_chunk] in Hofs. lia.
-        - apply Z.divide_0_r.
-      }
-      edestruct (Mem.valid_access_store m' Mint32 b 0) as (m'' & Hm'').
-      {
-        constructor.
-        - intros ofs Hofs. eapply Mem.perm_store_1; eauto.
-        - apply Z.divide_0_r.
-      }
-      eexists. split.
-      * eapply plus_left. cbn.
-        {
-          constructor; eauto.
-          repeat constructor. cbn. solve_list_disjoint.
-        }
-        lts_step. crush_step.
-        lts_step. crush_step.
-        lts_step. crush_step.
-        lts_step. crush_step. crush_expr.
-        lts_step. crush_step.
-        lts_step.
-        (* assign *)
-        crush_step; crush_expr. now constructor.
-        lts_step. crush_step.
-        (* assign *)
-        lts_step.
-        {
-          crush_step; crush_expr.
-          - erewrite Mem.load_store_same; eauto.
-          - apply cop_sem_mod. unfold Int.zero.
-            intros contra. inv contra.
-          - constructor. eauto.
-        }
-        lts_step. crush_step.
-        lts_step. crush_step; crush_expr. now constructor.
-        apply star_refl. reflexivity.
-      *
-        cbn. rewrite H6.
-        replace (Int.repr (Int.intval i)) with i by now rewrite Int.repr_unsigned.
-        constructor.
-        constructor.
-        (* c1 *)
-        -- econstructor; eauto.
-           ++ erewrite Mem.load_store_same; eauto.
-           ++ cbn. constructor.
-              apply cnt_inc_simp; assumption.
-           ++ apply Nat.mod_upper_bound. lia.
-           ++ intros ofs Hofs. eapply Mem.perm_store_1; eauto.
-              eapply Mem.perm_store_1; eauto.
-        (* c2 *)
-        -- cut (rel_cnt se2 cnt2_id c2 m'). intros X.
-           eapply rel_cnt_store_other; eauto. intros x. inv x.
-           eapply rel_cnt_store_other; eauto. intros x. inv x.
-        -- cut (rel_arr se2 f m'). intros X.
-           eapply rel_arr_store_other; eauto. intros x. inv x.
-           eapply rel_arr_store_other; eauto. intros x. inv x.
+    + eexists tt, _.  split. 2: split.
+      * econstructor; eauto.
+        eapply genv_funct_symbol; eauto. reflexivity.
+      * assert (b = b0). cbn in *. congruence.
+        subst. constructor.
+      * split. constructor. intros. inv H. inv H1.
+        eexists. split; constructor; eauto.
     (* inc2 *)
-    + inv H2. inv H8. inv H2.
-      edestruct (Mem.valid_access_store m Mint32 b 0) as (m' & Hm').
-      {
-        constructor.
-        - intros ofs Hofs. apply H5. cbn [size_chunk] in Hofs. lia.
-        - apply Z.divide_0_r.
-      }
-      edestruct (Mem.valid_access_store m' Mint32 b 0) as (m'' & Hm'').
-      {
-        constructor.
-        - intros ofs Hofs. eapply Mem.perm_store_1; eauto.
-        - apply Z.divide_0_r.
-      }
-      eexists. split.
-      * eapply plus_left. cbn.
-        {
-          constructor; eauto.
-          repeat constructor. cbn. solve_list_disjoint.
-        }
-        lts_step. crush_step.
-        lts_step. crush_step.
-        lts_step. crush_step.
-        lts_step. crush_step. crush_expr.
-        lts_step. crush_step.
-        lts_step.
-        (* assign *)
-        crush_step; crush_expr. now constructor.
-        lts_step. crush_step.
-        (* assign *)
-        lts_step.
-        {
-          crush_step; crush_expr.
-          - erewrite Mem.load_store_same; eauto.
-          - apply cop_sem_mod. unfold Int.zero.
-            intros contra. inv contra.
-          - constructor. eauto.
-        }
-        lts_step. crush_step.
-        lts_step. crush_step; crush_expr. now constructor.
-        apply star_refl. reflexivity.
-      *
-        cbn. rewrite H7.
-        replace (Int.repr (Int.intval i)) with i by now rewrite Int.repr_unsigned.
-        constructor.
-        constructor.
-        (* c1 *)
-        -- cut (rel_cnt se2 cnt1_id c1 m'). intros X.
-           eapply rel_cnt_store_other; eauto. intros x. inv x.
-           eapply rel_cnt_store_other; eauto. intros x. inv x.
-        (* c2 *)
-        -- econstructor; eauto.
-           ++ erewrite Mem.load_store_same; eauto.
-           ++ cbn. constructor.
-              apply cnt_inc_simp; assumption.
-           ++ apply Nat.mod_upper_bound. lia.
-           ++ intros ofs Hofs. eapply Mem.perm_store_1; eauto.
-              eapply Mem.perm_store_1; eauto.
-        -- cut (rel_arr se2 f m'). intros X.
-           eapply rel_arr_store_other; eauto. intros x. inv x.
-           eapply rel_arr_store_other; eauto. intros x. inv x.
-    (* set *)
-    + inv H2. inv H11.
-      edestruct (Mem.valid_access_store m Mint32 b (4 * Z.of_nat i)) as (m' & Hm').
-      {
-        constructor.
-        - intros ofs Hofs. apply H2. unfold Nz. split.
-          lia. cbn [size_chunk] in Hofs. unfold N in *. lia.
-        - apply Z.divide_factor_l.
-      }
-      eexists. split.
-      * eapply plus_left.
-        {
-          constructor; eauto. repeat constructor. cbn.
-          intros [A|A]; inv A. intros A. inv A. solve_list_disjoint.
-        }
-        lts_step. crush_step.
-        lts_step. crush_step; crush_expr.
-        {
-          match goal with
-          | [ H: Mem.store _ ?m ?b ?ofs ?v = Some ?m' |-
-              Mem.store _ ?m ?b ?ofs' ?v' = Some _ ] =>
-              replace ofs' with ofs; [ apply H | ]
-          end.
-          rewrite Ptrofs.add_zero_l.
-          unfold Ptrofs.of_intu, Ptrofs.of_int, Ptrofs.mul.
-          rewrite Int.unsigned_repr.
-          repeat rewrite Ptrofs.unsigned_repr.
-          all: pose proof Nbound; pose proof Nbound';
-            unfold Nz in *; unfold N in *; try lia.
-        }
-        lts_step. crush_step.
-        lts_step. crush_step; crush_expr.
-        apply star_refl. reflexivity.
-      * constructor. constructor.
-        -- eapply rel_cnt_store_other; eauto. intros x. inv x.
-        -- eapply rel_cnt_store_other; eauto. intros x. inv x.
-        -- econstructor; eauto. intros ix.
-           2: { intros ofs Hofs. eapply Mem.perm_store_1; eauto. }
-           destruct Nat.eq_dec.
-           ++ subst. intros. exists v2. split; auto.
-              erewrite Mem.load_store_same; eauto.
-              f_equal.
-              eapply val_casted_load_result; eauto.
-           ++ intros Hix. edestruct (H1 _ Hix) as (vx & Hvx & Hrv).
-              exists vx; split; auto.
-              erewrite Mem.load_store_other; eauto. right.
-              apply not_eq in n. destruct n.
-              ** right. apply inj_lt in H4. cbn [size_chunk]. lia.
-              ** left. apply inj_lt in H4. cbn [size_chunk]. lia.
+    + eexists tt, _.  split. 2: split.
+      * econstructor; eauto.
+        eapply genv_funct_symbol; eauto. reflexivity.
+      * assert (b = b0).  cbn in *. congruence.
+        subst. constructor.
+      * split. constructor. intros. inv H. inv H1.
+        eexists. split; constructor; eauto.
     (* get *)
-    + inv H2. inv H10. edestruct (H1 _ H9) as (vx & Hvx & Hvr & Hrt).
+    + eexists tt, _.  split. 2: split.
+      * econstructor; eauto.
+        eapply genv_funct_symbol; eauto. reflexivity.
+      * assert (b = b0). cbn in *. congruence.
+        subst. constructor.
+      * split. constructor. intros. inv H. inv H1.
+        eexists. split. econstructor; eauto.
+        econstructor. apply H8. apply H6. reflexivity.
+    (* set *)
+    + eexists tt, _.  split. 2: split.
+      * econstructor; eauto.
+        eapply genv_funct_symbol; eauto. reflexivity.
+      * assert (b = b0). cbn in *. congruence.
+        subst. constructor.
+      * split. constructor. intros. inv H. inv H1.
+        eexists. split. econstructor; eauto.
+        econstructor. reflexivity.
+  - intros. inv H1; inv H.
+    (* enq: from initial to call inc2 *)
+    + exploit inc2_block; eauto. intros (b1 & A & B).
       eexists. split.
-      * eapply plus_left.
+      * eapply plus_left. constructor; eauto.
         {
-          constructor; eauto. repeat constructor. cbn.
-          easy. solve_list_disjoint.
+          constructor; repeat constructor.
+          intros x. inv x. solve_list_disjoint.
         }
+        lts_step. crush_step.
         lts_step. crush_step; crush_expr.
-        {
-          match goal with
-          | [ H: Mem.load _ ?m ?b ?ofs = Some _ |- Mem.load _ ?m ?b ?ofs' = Some _ ] =>
-              replace ofs' with ofs; [ apply H | ]
-          end.
-          unfold Ptrofs.of_intu, Ptrofs.of_int, Ptrofs.mul.
-          rewrite Ptrofs.add_zero_l.
-          rewrite Int.unsigned_repr.
-          repeat rewrite Ptrofs.unsigned_repr.
-          all: pose proof Nbound; pose proof Nbound';
-            unfold Nz in *; unfold N in *; try lia.
-        }
         apply star_refl. reflexivity.
-      * subst. constructor. constructor; eauto. econstructor; eauto.
+      * econstructor; eauto.
+    (* deq: from initial to call inc1 *)
+    + exploit inc1_block; eauto. intros (b1 & A & B).
+      eexists. split.
+      * eapply plus_left. constructor; eauto.
+        { constructor; repeat constructor. solve_list_disjoint. }
+        lts_step. crush_step.
+        lts_step. crush_step; crush_expr.
+        apply star_refl. reflexivity.
+      * econstructor; eauto.
+    (* enq: after inc2, call set *)
+    + exploit set_block; eauto. intros (b1 & A & B).
+      eexists. split.
+      * eapply plus_left. constructor; eauto.
+        lts_step. crush_step.
+        lts_step. crush_step.
+        lts_step. crush_step; crush_expr.
+        apply star_refl. reflexivity.
+      * econstructor; eauto.
+    (* deq: after inc1, call get *)
+    + exploit get_block; eauto. intros (b1 & A & B).
+      eexists. split.
+      * eapply plus_left. constructor; eauto.
+        lts_step. crush_step.
+        lts_step. crush_step.
+        lts_step. crush_step; crush_expr.
+        apply star_refl. reflexivity.
+      * econstructor; eauto.
+    (* enq: to final state *)
+    + eexists. split.
+      * eapply plus_left. constructor.
+        lts_step. crush_step.
+        lts_step. crush_step; crush_expr.
+        apply star_refl. reflexivity.
+      * constructor.
+    (* deq: to final state *)
+    + eexists. split.
+      * eapply plus_left. constructor.
+        lts_step. crush_step.
+        lts_step. crush_step; crush_expr.
+        apply star_refl. reflexivity.
+      * constructor.
   - apply well_founded_ltof.
 Qed.
